adjusted to new sting constants, fixed some minor issues.

gravy/src/org/gravy/GlobalsCache.java
@@ -10,10 +10,6 @@ import boogie.ProgramFactory;
  *
  */
 public class GlobalsCache {
-
-	public static final String cloneAttribute = "ClonedBlock";
-	
-	public static final String ignoreInfeasibleReport = "IgnoreReport";
 	
 	private static GlobalsCache instance = null;
 	
