gravy/test/out.bpl
@@ -2,59 +2,174 @@ type ref;
 type javaType;
 type Field $GenericType__0;
 type $heap_type = <$GenericType__0>[ref,Field $GenericType__0]$GenericType__0;
-
+type boolArrHeap_type = [ref][int]bool;
+type refArrHeap_type = [ref][int]ref;
+type realArrHeap_type = [ref][int]int;
+type intArrHeap_type = [ref][int]int;
 const unique $type : Field javaType;
 const unique $alloc : Field bool;
 const unique $null : ref;
 const { :sourceloc "Object.java",-1,-1,-1,-1 } unique java.lang.Object : javaType extends  complete;
-const { :sourceloc "FalsePositives03.java",-1,-1,-1,-1 } unique FalsePositives03 : javaType extends  unique java.lang.Object complete;
-const { :sourceloc "Context.java",-1,-1,-1,-1 } unique javax.naming.Context : javaType extends  unique java.lang.Object complete;
+const { :sourceloc "FalsePositives04.java",-1,-1,-1,-1 } unique FalsePositives04 : javaType extends  unique java.lang.Object complete;
+const { :sourceloc "Serializable.java",-1,-1,-1,-1 } unique java.io.Serializable : javaType extends  unique java.lang.Object complete;
+const { :sourceloc "Throwable.java",-1,-1,-1,-1 } unique java.lang.Throwable : javaType extends  unique java.io.Serializable, unique java.lang.Object complete;
+const { :sourceloc "Exception.java",-1,-1,-1,-1 } unique java.lang.Exception : javaType extends  unique java.lang.Throwable complete;
+const { :sourceloc "RuntimeException.java",-1,-1,-1,-1 } unique java.lang.RuntimeException : javaType extends  unique java.lang.Exception complete;
+const { :sourceloc "NullPointerException.java",-1,-1,-1,-1 } unique java.lang.NullPointerException : javaType extends  unique java.lang.RuntimeException complete;
+const { :sourceloc "Comparable.java",-1,-1,-1,-1 } unique java.lang.Comparable : javaType extends  unique java.lang.Object complete;
+const { :sourceloc "CharSequence.java",-1,-1,-1,-1 } unique java.lang.CharSequence : javaType extends  unique java.lang.Object complete;
+const { :sourceloc "String.java",-1,-1,-1,-1 } unique java.lang.String : javaType extends  unique java.io.Serializable, unique java.lang.CharSequence, unique java.lang.Comparable, unique java.lang.Object complete;
 var $heap : $heap_type;
-
-
+var $intArrayType : javaType;
+var $charArrayType : javaType;
+var $boolArrayType : javaType;
+var $byteArrayType : javaType;
+var $longArrayType : javaType;
+var $arrSizeHeap : [ref]int;
+var $stringSizeHeap : [ref]int;
+var $boolArrHeap : boolArrHeap_type;
+var $refArrHeap : refArrHeap_type;
+var $realArrHeap : realArrHeap_type;
+var $intArrHeap : intArrHeap_type;
+var java.lang.Object$FalsePositives04$first234 : Field ref;
+function $arrayType(t:javaType) returns ($ret:javaType);
 function $intToReal(x:int) returns ($ret:real);
 function $intToBool(x:int) returns ($ret:bool) { (if x == 0 then false else true) }
 function $refToBool(x:ref) returns ($ret:bool) { (if x == $null then false else true) }
 function $boolToInt(x:bool) returns ($ret:int) { (if x == true then 1 else 0) }
+function $cmpBool(x:bool, y:bool) returns ($ret:int);
+function $cmpRef(x:ref, y:ref) returns ($ret:int);
+function $cmpReal(x:real, y:real) returns ($ret:int) { (if x > y then 1 else (if x < y then -1 else 0)) }
+function $cmpInt(x:int, y:int) returns ($ret:int) { (if x > y then 1 else (if x < y then -1 else 0)) }
+function $bitOr(x:int, y:int) returns ($ret:int);
+function $bitAnd(x:int, y:int) returns ($ret:int);
+function $xorInt(x:int, y:int) returns ($ret:int);
+function $shlInt(x:int, y:int) returns ($ret:int);
+function $ushrInt(x:int, y:int) returns ($ret:int);
+function $shrInt(x:int, y:int) returns ($ret:int);
+axiom (forall t : javaType :: $heap[$null,$type] <: t);
+procedure $new(obj_type:javaType) returns ($obj:ref);    ensures $heap[$obj,$type] == obj_type;    requires $heap[$obj,$alloc] == false;        ensures $obj != $null;    ensures $heap[$obj,$alloc] == true;
 
+procedure java.lang.Object$java.lang.Object$clone$43($this:ref) returns ($other:ref);        ensures $other != $null;    ensures $heap[$other,$alloc] == true;    ensures $heap[$other,$type] == $heap[$this,$type];
 
+procedure int$java.lang.String$compareTo$87($this:ref, $other:ref) returns ($return:int);    
 
+procedure java.lang.Object$FalsePositives04$peekFirst$1890($this:ref) returns ($return:ref, $exception:ref);    modifies $heap;
 
-procedure void$FalsePositives03$foo$1889($this:ref, $in_parameter__0:ref) returns ($exception:ref);    
+procedure java.lang.Object$FalsePositives04$foo$1889($this:ref) returns ($return:ref, $exception:ref);    modifies $heap;
 
+procedure java.lang.String$java.lang.Object$toString$44($this:ref) returns ($return:ref, $exception:ref);    
 
-implementation void$FalsePositives03$foo$1889($this:ref, $in_parameter__0:ref) returns ($exception:ref){
+procedure void$FalsePositives04$$la$init$ra$$1891($this:ref) returns ($exception:ref);    
+
+procedure void$java.lang.Object$$la$init$ra$$38($this:ref) returns ($exception:ref);    
+
+implementation java.lang.Object$FalsePositives04$peekFirst$1890($this:ref) returns ($return:ref, $exception:ref){
     
-var temp$03 : int;    
-var ctx4 : ref;    
+var temp$24 : ref;    
 var this1 : ref;    
-var container2 : ref;
+var temp$35 : ref;    
+var temp$13 : ref;    
+var temp$68 : ref;    
+var temp$57 : ref;    
+var temp$79 : ref;    
+var temp$02 : ref;    
+var temp$46 : ref;
     assume $this != $null;
+    assume $heap[$return,$type] <: java.lang.Object;
+    assert { :sourceloc "FalsePositives04.java",8,5,17,5 } true;
     this1 := $this;
-    container2 := $in_parameter__0;
-    temp$03 := $boolToInt($heap[container2,$type] <: javax.naming.Context);
-    if (temp$03 == 0) {
-        assert { :sourceloc "FalsePositives03.java",15,13,15,40 } true;
-        goto block1;
-    } else {
-        assert { :sourceloc "FalsePositives03.java",15,13,15,40 } true;
-    }
-    goto block2;
   block1:
-    if (container2 == $null) {
-        assert { :sourceloc "FalsePositives03.java",15,45,15,61 } true;
+    assert { :sourceloc "FalsePositives04.java",8,5,17,5 } true;
+    assert { :sourceloc "FalsePositives04.java",10,18,10,22 } true;
+    call temp$02, $exception := java.lang.Object$FalsePositives04$foo$1889(this1);
+    if ($exception != $null && $heap[$exception,$type] <: java.lang.Throwable) {
         goto block2;
-    } else {
-        assert { :sourceloc "FalsePositives03.java",15,45,15,61 } true;
     }
-    goto block3;
-    goto block3;
-  block2:
-    assert { :sourceloc "FalsePositives03.java",16,13,16,48 } $heap[container2,$type] <: javax.naming.Context;
-    ctx4 := container2;
-    goto block4;
+    assert { :sourceloc "FalsePositives04.java",10,10,10,14 } true;
+    $heap := $heap[this1,java.lang.Object$FalsePositives04$first234 := temp$02];
+    assert { :sourceloc "FalsePositives04.java",11,20,11,24 } true;
+    temp$13 := $heap[this1,java.lang.Object$FalsePositives04$first234];
+    assert { :sourceloc "FalsePositives04.java",11,20,11,24 } true;
+    if (temp$13 != $null) {
+        assert { :sourceloc "FalsePositives04.java",11,20,11,24 } true;
+    } else {
+        assert { :noverify } true;
+        call $exception := $new(java.lang.NullPointerException);
+        goto block2;
+    }
+    call temp$24, $exception := java.lang.String$java.lang.Object$toString$44(temp$13);
+    if ($exception != $null && $heap[$exception,$type] <: java.lang.Throwable) {
+        goto block2;
+    }
   block3:
+    assert { :sourceloc "FalsePositives04.java",11,20,11,24 } true;
+    assert { :sourceloc "FalsePositives04.java",13,14,13,18 } { :clone } true;
+    assert { :sourceloc "FalsePositives04.java",13,14,13,18 } { :clone } this1 != $null;
+    temp$35 := $heap[this1,java.lang.Object$FalsePositives04$first234];
+    assert { :sourceloc "FalsePositives04.java",13,14,13,18 } { :clone } true;
+    if (temp$35 == $null) {
+        assert { :sourceloc "FalsePositives04.java",13,14,13,18 } { :clone } true;
+        goto block4;
+    } else {
+        assert { :sourceloc "FalsePositives04.java",13,14,13,18 } { :clone } true;
+    }
+    assert { :sourceloc "FalsePositives04.java",13,14,13,18 } { :clone } true;
+    goto block5;
   block4:
+    assert { :sourceloc "FalsePositives04.java",13,14,13,18 } { :clone } true;
+    assert { :sourceloc "FalsePositives04.java",13,14,13,18 } { :clone } true;
+    temp$46 := $null;
+    assert { :sourceloc "FalsePositives04.java",14,11,14,22 } true;
+    $return := temp$46;
+    return;
+  block5:
+    assert { :sourceloc "FalsePositives04.java",14,11,14,22 } true;
+    assert { :sourceloc "FalsePositives04.java",11,13,11,36 } true;
+    $return := temp$24;
+    return;
+  block2:
+    assert { :sourceloc "FalsePositives04.java",11,13,11,36 } true;
+    assert { :sourceloc "FalsePositives04.java",9,9,16,9 } true;
+    assert { :sourceloc "FalsePositives04.java",9,9,16,9 } $exception != $null;
+    assume $heap[$exception,$type] <: java.lang.Throwable;
+    temp$57 := $exception;
+    assert { :sourceloc "FalsePositives04.java",13,14,13,18 } { :clone } true;
+    assert { :sourceloc "FalsePositives04.java",13,14,13,18 } { :clone } this1 != $null;
+    temp$68 := $heap[this1,java.lang.Object$FalsePositives04$first234];
+    assert { :sourceloc "FalsePositives04.java",13,14,13,18 } { :clone } true;
+    if (temp$68 == $null) {
+        assert { :sourceloc "FalsePositives04.java",13,14,13,18 } { :clone } true;
+        goto block6;
+    } else {
+        assert { :sourceloc "FalsePositives04.java",13,14,13,18 } { :clone } true;
+    }
+    assert { :sourceloc "FalsePositives04.java",13,14,13,18 } { :clone } true;
+    goto block7;
+  block6:
+    assert { :sourceloc "FalsePositives04.java",13,14,13,18 } { :clone } true;
+    assert { :sourceloc "FalsePositives04.java",13,14,13,18 } { :clone } true;
+    temp$79 := $null;
+    assert { :sourceloc "FalsePositives04.java",14,11,14,22 } true;
+    $return := temp$79;
+    return;
+  block7:
+    assert { :sourceloc "FalsePositives04.java",14,11,14,22 } true;
+    assert { :sourceloc "FalsePositives04.java",14,11,14,22 } true;
+    $exception := temp$57;
+    return;
+}
+
+
+implementation void$FalsePositives04$$la$init$ra$$1891($this:ref) returns ($exception:ref){
+    
+var this10 : ref;
+    assume $this != $null;
+    assert { :sourceloc "FalsePositives04",3,-1,-1,-1 } true;
+    this10 := $this;
+    assert { :sourceloc "FalsePositives04",3,-1,-1,-1 } true;
+    call $exception := void$java.lang.Object$$la$init$ra$$38(this10);
+    assert { :sourceloc "FalsePositives04",3,-1,-1,-1 } true;
     return;
 }
 
